SeparationLogic/DownUpSemantics_Fail.v
@@ -12,18 +12,7 @@ Local Open Scope PropositionalLogic.
 Local Open Scope SeparationLogic.
 Local Open Scope KripkeSemantics.
 
-Class DownUpSemantics (L: Language) {nL: NormalLanguage L} {pL: PropositionalLanguage L} {SL: SeparationLanguage L} (SM: Semantics L) {pkSM: PreKripkeSemantics L SM} {kiM: KripkeIntuitionisticModel L SM} {kiSM: KripkeIntuitionisticSemantics L SM} : Type := {
-  join: forall {M: Kmodel}, Kworlds M -> Kworlds M -> Kworlds M -> Prop;
-  join_comm: forall M (m1 m2 m: Kworlds M), join m1 m2 m -> join m2 m1 m;
-  join_assoc: forall M (mx my mz mxy mxyz: Kworlds M), join mx my mxy -> join mxy mz mxyz -> exists myz, join my mz myz /\ join mx myz mxyz;
-  sat_sepcon: forall M m x y, KRIPKE: M , m |= x * y <-> exists m0 m1 m2, Korder m m0 /\ join m1 m2 m0 /\ KRIPKE: M , m1 |= x /\ KRIPKE: M, m2 |= y;
-  sat_wand: forall M m x y, KRIPKE: M , m |= x -* y <-> forall m0 m1 m2, Korder m0 m -> join m1 m0 m2 -> KRIPKE: M , m1 |= x -> KRIPKE: M, m2 |= y
+Class DownUpSemantics (L: Language) {nL: NormalLanguage L} {pL: PropositionalLanguage L} {SL: SeparationLanguage L} (MD: Model) {kMD: KripkeModel MD} (M: Kmodel) {kiM: KripkeIntuitionisticModel MD M} {SA: SeparationAlgebra MD M} (SM: Semantics L MD) {kiSM: KripkeIntuitionisticSemantics L MD M SM}: Type := {
+  sat_sepcon: forall m x y, KRIPKE: M , m |= x * y <-> exists m0 m1 m2, m <= m0 /\ join m1 m2 m0 /\ KRIPKE: M , m1 |= x /\ KRIPKE: M, m2 |= y;
+  sat_wand: forall m x y, KRIPKE: M , m |= x -* y <-> forall m0 m1 m2, m0 <= m -> join m1 m0 m2 -> KRIPKE: M , m1 |= x -> KRIPKE: M, m2 |= y
 }.
-
-(*
-
-  sat_sepcon: forall M m x y, KRIPKE: M , m |= x * y <-> exists m1 m2, join m1 m2 m /\ KRIPKE: M , m1 |= x /\ KRIPKE: M, m2 |= y;
-  sat_wand: forall M m x y, KRIPKE: M , m |= x -* y <-> forall m1 m2, join m1 m m2 -> KRIPKE: M , m1 |= x -> KRIPKE: M, m2 |= y
-
-*)
-
