SeparationLogic/DownwardsSemantics.v
@@ -11,21 +11,21 @@ Local Open Scope PropositionalLogic.
 Local Open Scope KripkeSemantics.
 Local Open Scope SeparationLogic.
 
-Class DownwardsClosedSeparationAlgebra (MD: Model) {kMD: KripkeModel MD} {kiMD: KripkeIntuitionisticModel MD} {SA: SeparationAlgebra MD} (M: Kmodel): Type := {
+Class DownwardsClosedSeparationAlgebra (MD: Model) {kMD: KripkeModel MD} (M: Kmodel) {kiM: KripkeIntuitionisticModel MD M} {SA: SeparationAlgebra MD M}: Type := {
   join_Korder_down: forall (m n m1 m2: Kworlds M), join m1 m2 m -> n <= m -> exists n1 n2, join n1 n2 n /\ n1 <= m1 /\ n2 <= m2
 }.
 
-Class DownwardsSemantics (L: Language) {nL: NormalLanguage L} {pL: PropositionalLanguage L} {SL: SeparationLanguage L} (MD: Model) {kMD: KripkeModel MD} {kiMD: KripkeIntuitionisticModel MD} {SA: SeparationAlgebra MD} (SM: Semantics L MD) {kiSM: KripkeIntuitionisticSemantics L MD SM}: Type := {
-  sat_sepcon: forall M m x y, KRIPKE: M , m |= x * y <-> exists m1 m2, join m1 m2 m /\ KRIPKE: M , m1 |= x /\ KRIPKE: M, m2 |= y;
-  sat_wand: forall M m x y, KRIPKE: M , m |= x -* y <-> forall m0 m1 m2, m0 <= m -> join m0 m1 m2 -> KRIPKE: M , m1 |= x -> KRIPKE: M, m2 |= y
+Class DownwardsSemantics (L: Language) {nL: NormalLanguage L} {pL: PropositionalLanguage L} {SL: SeparationLanguage L} (MD: Model) {kMD: KripkeModel MD} (M: Kmodel) {kiM: KripkeIntuitionisticModel MD M} {SA: SeparationAlgebra MD M} (SM: Semantics L MD) {kiSM: KripkeIntuitionisticSemantics L MD M SM}: Type := {
+  sat_sepcon: forall m x y, KRIPKE: M , m |= x * y <-> exists m1 m2, join m1 m2 m /\ KRIPKE: M , m1 |= x /\ KRIPKE: M, m2 |= y;
+  sat_wand: forall m x y, KRIPKE: M , m |= x -* y <-> forall m0 m1 m2, m0 <= m -> join m0 m1 m2 -> KRIPKE: M , m1 |= x -> KRIPKE: M, m2 |= y
 }.
 
-Class DownwardsClosedUnitarySeparationAlgebra (MD: Model) {kMD: KripkeModel MD} {kiMD: KripkeIntuitionisticModel MD} {SA: SeparationAlgebra MD} {USA: UnitarySeparationAlgebra MD} (M: Kmodel): Type := {
+Class DownwardsClosedUnitarySeparationAlgebra (MD: Model) {kMD: KripkeModel MD} (M: Kmodel) {kiM: KripkeIntuitionisticModel MD M} {SA: SeparationAlgebra MD M} {USA: UnitarySeparationAlgebra MD M}: Type := {
   unit_spec : forall m: Kworlds M, unit m <-> forall n n', join m n n' -> n' <= n;
   unit_exists: forall n: Kworlds M, exists m, join m n n /\ (forall m', m' <= m -> unit m')
 }.
 
-Class UnitaryDownwardsSemantics (L: Language) {nL: NormalLanguage L} {pL: PropositionalLanguage L} {SL: SeparationLanguage L} {uSL: UnitarySeparationLanguage L} (MD: Model) {kMD: KripkeModel MD} {kiMD: KripkeIntuitionisticModel MD} {SA: SeparationAlgebra MD} {USA: UnitarySeparationAlgebra MD} (SM: Semantics L MD) {kiSM: KripkeIntuitionisticSemantics L MD SM} {dsSM: DownwardsSemantics L MD SM}: Type := {
-  sat_emp: forall M (m: Kworlds M), KRIPKE: M, m |= emp <-> forall n, n <= m -> unit n
+Class UnitaryDownwardsSemantics (L: Language) {nL: NormalLanguage L} {pL: PropositionalLanguage L} {SL: SeparationLanguage L} {uSL: UnitarySeparationLanguage L} (MD: Model) {kMD: KripkeModel MD} (M: Kmodel) {kiM: KripkeIntuitionisticModel MD M} {SA: SeparationAlgebra MD M} {USA: UnitarySeparationAlgebra MD M} (SM: Semantics L MD) {kiSM: KripkeIntuitionisticSemantics L MD M SM} {dsSM: DownwardsSemantics L MD M SM}: Type := {
+  sat_emp: forall (m: Kworlds M), KRIPKE: M, m |= emp <-> forall n, n <= m -> unit n
 }.
 
