SeparationLogic/Downwards2Upwards.v
@@ -5,12 +5,14 @@ Require Import Logic.MinimunLogic.MinimunLogic.
 Require Import Logic.PropositionalLogic.Syntax.
 Require Import Logic.SeparationLogic.Syntax.
 Require Import Logic.PropositionalLogic.KripkeSemantics.
+Require Import Logic.SeparationLogic.SeparationAlgebra.
 Require Import Logic.SeparationLogic.DownwardsSemantics.
 Require Import Logic.SeparationLogic.UpwardsSemantics.
 
 Local Open Scope logic_base.
 Local Open Scope PropositionalLogic.
 Local Open Scope SeparationLogic.
+Local Open Scope KripkeSemantics.
 
 Definition d2u_sSM {L: Language} {nL: NormalLanguage L} {pL: PropositionalLanguage L} {SL: SeparationLanguage L} {SM: Semantics L} {pkSM: PreKripkeSemantics L SM} {kiM: KripkeIntuitionisticModel L SM} {kiSM: KripkeIntuitionisticSemantics L SM} (dsSM: DownwardsSemantics L SM): UpwardsSemantics L SM.
   refine (Build_UpwardsSemantics _ _ _ _ _ _ _ _ (fun M (m1 m2 m: Kworlds M) => exists n1 n2, Korder n1 m1 /\ Korder n2 m2 /\ DownwardsSemantics.join n1 n2 m) _ _ _ _ _).
