SeparationLogic/Sound_DownUp_Fail.v
@@ -5,6 +5,7 @@ Require Import Logic.MinimunLogic.MinimunLogic.
 Require Import Logic.PropositionalLogic.Syntax.
 Require Import Logic.SeparationLogic.Syntax.
 Require Import Logic.PropositionalLogic.KripkeSemantics.
+Require Import Logic.SeparationLogic.SeparationAlgebra.
 Require Import Logic.SeparationLogic.DownUpSemantics_Fail.
 Require Import Logic.PropositionalLogic.IntuitionisticPropositionalLogic.
 Require Import Logic.SeparationLogic.SeparationLogic.
@@ -12,14 +13,15 @@ Require Import Logic.SeparationLogic.SeparationLogic.
 Local Open Scope logic_base.
 Local Open Scope PropositionalLogic.
 Local Open Scope SeparationLogic.
+Local Open Scope KripkeSemantics.
 
-Lemma sound_sepcon_comm {L: Language} {nL: NormalLanguage L} {pL: PropositionalLanguage L} {SL: SeparationLanguage L} {SM: Semantics L} {pkS: PreKripkeSemantics L SM} {kiM: KripkeIntuitionisticModel L SM} {kiSM: KripkeIntuitionisticSemantics L SM} {dusSM: DownUpSemantics L SM}:
+Lemma sound_sepcon_comm {L: Language} {nL: NormalLanguage L} {pL: PropositionalLanguage L} {SL: SeparationLanguage L} {MD: Model} {kMD: KripkeModel MD} (M: Kmodel) {kiM: KripkeIntuitionisticModel MD M} {SA: SeparationAlgebra MD M} {SM: Semantics L MD} {kiSM: KripkeIntuitionisticSemantics L MD M SM} {dusSM: DownUpSemantics L MD M SM}:
   forall x y: expr,
-    forall M m,
+    forall m,
       KRIPKE: M, m |= x * y --> y * x.
 Proof.
   intros.
-  pose proof Korder_PreOrder M as H_PreOrder.
+  pose proof Korder_PreOrder as H_PreOrder.
   rewrite sat_impp; intros.
   rewrite sat_sepcon in H0 |- *; intros.
   destruct H0 as [m0 [m1 [m2 [? [? [? ?]]]]]].
@@ -28,9 +30,9 @@ Proof.
   apply join_comm; auto.
 Qed.
 
-Lemma sound_sepcon_assoc {L: Language} {nL: NormalLanguage L} {pL: PropositionalLanguage L} {SL: SeparationLanguage L} {SM: Semantics L} {pkS: PreKripkeSemantics L SM} {kiM: KripkeIntuitionisticModel L SM} {kiSM: KripkeIntuitionisticSemantics L SM} {dusSM: DownUpSemantics L SM}:
+Lemma sound_sepcon_assoc {L: Language} {nL: NormalLanguage L} {pL: PropositionalLanguage L} {SL: SeparationLanguage L} {MD: Model} {kMD: KripkeModel MD} (M: Kmodel) {kiM: KripkeIntuitionisticModel MD M} {SA: SeparationAlgebra MD M} {SM: Semantics L MD} {kiSM: KripkeIntuitionisticSemantics L MD M SM} {dusSM: DownUpSemantics L MD M SM}:
   forall x y z: expr,
-    forall M m,
+    forall m,
       KRIPKE: M, m |= x * (y * z) <--> (x * y) * z.
 Proof.
   intros.
