SeparationLogic/Sound_Downwards.v
@@ -5,6 +5,7 @@ Require Import Logic.MinimunLogic.MinimunLogic.
 Require Import Logic.PropositionalLogic.Syntax.
 Require Import Logic.SeparationLogic.Syntax.
 Require Import Logic.PropositionalLogic.KripkeSemantics.
+Require Import Logic.SeparationLogic.SeparationAlgebra.
 Require Import Logic.SeparationLogic.DownwardsSemantics.
 Require Import Logic.PropositionalLogic.IntuitionisticPropositionalLogic.
 Require Import Logic.SeparationLogic.SeparationLogic.
@@ -12,10 +13,11 @@ Require Import Logic.SeparationLogic.SeparationLogic.
 Local Open Scope logic_base.
 Local Open Scope PropositionalLogic.
 Local Open Scope SeparationLogic.
+Local Open Scope KripkeSemantics.
 
-Lemma sound_sepcon_comm {L: Language} {nL: NormalLanguage L} {pL: PropositionalLanguage L} {SL: SeparationLanguage L} {SM: Semantics L} {pkS: PreKripkeSemantics L SM} {kiM: KripkeIntuitionisticModel L SM} {kiSM: KripkeIntuitionisticSemantics L SM} {dsSM: DownwardsSemantics L SM}:
+Lemma sound_sepcon_comm {L: Language} {nL: NormalLanguage L} {pL: PropositionalLanguage L} {SL: SeparationLanguage L} {MD: Model} {kMD: KripkeModel MD} (M: Kmodel) {kiM: KripkeIntuitionisticModel MD M} {SA: SeparationAlgebra MD M} {SM: Semantics L MD} {kiSM: KripkeIntuitionisticSemantics L MD M SM} {dsSM: DownwardsSemantics L MD M SM}:
   forall x y: expr,
-    forall M m,
+    forall m,
       KRIPKE: M, m |= x * y --> y * x.
 Proof.
   intros.
@@ -27,9 +29,9 @@ Proof.
   apply join_comm; auto.
 Qed.
 
-Lemma sound_sepcon_assoc {L: Language} {nL: NormalLanguage L} {pL: PropositionalLanguage L} {sL: SeparationLanguage L} {SM: Semantics L} {pkS: PreKripkeSemantics L SM} {kiM: KripkeIntuitionisticModel L SM} {kiSM: KripkeIntuitionisticSemantics L SM} {dsSM: DownwardsSemantics L SM}:
+Lemma sound_sepcon_assoc {L: Language} {nL: NormalLanguage L} {pL: PropositionalLanguage L} {SL: SeparationLanguage L} {MD: Model} {kMD: KripkeModel MD} (M: Kmodel) {kiM: KripkeIntuitionisticModel MD M} {SA: SeparationAlgebra MD M} {SM: Semantics L MD} {kiSM: KripkeIntuitionisticSemantics L MD M SM} {dsSM: DownwardsSemantics L MD M SM}:
   forall x y z: expr,
-    forall M m,
+    forall m,
       KRIPKE: M, m |= x * (y * z) <--> (x * y) * z.
 Proof.
   intros.
@@ -43,7 +45,7 @@ Proof.
     destruct H2 as [my [mz [? [? ?]]]].
     apply join_comm in H0.
     apply join_comm in H2.
-    destruct (join_assoc _ mz my mx myz n H2 H0) as [mxy [? ?]].
+    destruct (join_assoc mz my mx myz n H2 H0) as [mxy [? ?]].
     apply join_comm in H5.
     apply join_comm in H6.
     rewrite sat_sepcon.
@@ -57,7 +59,7 @@ Proof.
     destruct H0 as [mxy [mz [? [? ?]]]].
     rewrite sat_sepcon in H1.
     destruct H1 as [mx [my [? [? ?]]]].
-    destruct (join_assoc _ mx my mz mxy n H1 H0) as [myz [? ?]].
+    destruct (join_assoc mx my mz mxy n H1 H0) as [myz [? ?]].
     rewrite sat_sepcon.
     exists mx, myz.
     split; [| split]; auto.
@@ -66,13 +68,12 @@ Proof.
     split; [| split]; auto.
 Qed.
 
-Lemma sound_wand_sepcon_adjoint {L: Language} {nL: NormalLanguage L} {pL: PropositionalLanguage L} {sL: SeparationLanguage L} {SM: Semantics L} {pkS: PreKripkeSemantics L SM} {kiM: KripkeIntuitionisticModel L SM} {kiSM: KripkeIntuitionisticSemantics L SM} {dsSM: DownwardsSemantics L SM}:
+Lemma sound_wand_sepcon_adjoint {L: Language} {nL: NormalLanguage L} {pL: PropositionalLanguage L} {SL: SeparationLanguage L} {MD: Model} {kMD: KripkeModel MD} (M: Kmodel) {kiM: KripkeIntuitionisticModel MD M} {SA: SeparationAlgebra MD M} {SM: Semantics L MD} {kiSM: KripkeIntuitionisticSemantics L MD M SM} {dsSM: DownwardsSemantics L MD M SM}:
   forall x y z: expr,
-    forall M,
-     (forall m, KRIPKE: M, m |= x * y --> z) <-> (forall m, KRIPKE: M, m |= x --> (y -* z)).
+    (forall m, KRIPKE: M, m |= x * y --> z) <-> (forall m, KRIPKE: M, m |= x --> (y -* z)).
 Proof.
   intros.
-  pose proof Korder_PreOrder M as H_PreOrder.
+  pose proof Korder_PreOrder as H_PreOrder.
   split; intro.
   + assert (ASSU: forall m1 m2 m, join m1 m2 m -> KRIPKE: M, m1 |= x -> KRIPKE: M, m2 |= y -> KRIPKE: M, m |= z).
     Focus 1. {
@@ -106,15 +107,14 @@ Proof.
     reflexivity.
 Qed.
 
-Lemma sound_sepcon_mono {L: Language} {nL: NormalLanguage L} {pL: PropositionalLanguage L} {sL: SeparationLanguage L} {SM: Semantics L} {pkS: PreKripkeSemantics L SM} {kiM: KripkeIntuitionisticModel L SM} {kiSM: KripkeIntuitionisticSemantics L SM} {dsSM: DownwardsSemantics L SM}:
+Lemma sound_sepcon_mono {L: Language} {nL: NormalLanguage L} {pL: PropositionalLanguage L} {SL: SeparationLanguage L} {MD: Model} {kMD: KripkeModel MD} (M: Kmodel) {kiM: KripkeIntuitionisticModel MD M} {SA: SeparationAlgebra MD M} {SM: Semantics L MD} {kiSM: KripkeIntuitionisticSemantics L MD M SM} {dsSM: DownwardsSemantics L MD M SM}:
   forall x1 x2 y1 y2: expr,
-    forall M,
-     (forall m, KRIPKE: M, m |= x1 --> x2) ->
-     (forall m, KRIPKE: M, m |= y1 --> y2) ->
-     (forall m, KRIPKE: M, m |= x1 * y1 --> x2 * y2).
+   (forall m, KRIPKE: M, m |= x1 --> x2) ->
+   (forall m, KRIPKE: M, m |= y1 --> y2) ->
+   (forall m, KRIPKE: M, m |= x1 * y1 --> x2 * y2).
 Proof.
   intros.
-  pose proof Korder_PreOrder M as H_PreOrder.
+  pose proof Korder_PreOrder as H_PreOrder.
   assert (ASSUx: forall m, KRIPKE: M, m |= x1 -> KRIPKE: M, m |= x2).
   Focus 1. {
     intros.
@@ -135,12 +135,12 @@ Proof.
   exists m1, m2; auto.
 Qed.
 
-Lemma sound_sepcon_emp {L: Language} {nL: NormalLanguage L} {pL: PropositionalLanguage L} {sL: SeparationLanguage L} {uSL: UnitarySeparationLanguage L} {SM: Semantics L} {pkS: PreKripkeSemantics L SM} {kiM: KripkeIntuitionisticModel L SM} {kiSM: KripkeIntuitionisticSemantics L SM} {dsSM: DownwardsSemantics L SM} {UdsSM: UnitaryDownwardsSemantics L SM}:
+Lemma sound_sepcon_emp {L: Language} {nL: NormalLanguage L} {pL: PropositionalLanguage L} {SL: SeparationLanguage L} {uSL: UnitarySeparationLanguage L} {MD: Model} {kMD: KripkeModel MD} (M: Kmodel) {kiM: KripkeIntuitionisticModel MD M} {SA: SeparationAlgebra MD M} {USA: UnitarySeparationAlgebra MD M} {dUSA: DownwardsClosedUnitarySeparationAlgebra MD M} {SM: Semantics L MD} {kiSM: KripkeIntuitionisticSemantics L MD M SM} {dsSM: DownwardsSemantics L MD M SM} {dUsSM: UnitaryDownwardsSemantics L MD M SM}:
   forall x: expr,
-    forall M m, KRIPKE: M, m |= x * emp <--> x.
+    forall m, KRIPKE: M, m |= x * emp <--> x.
 Proof.
   intros.
-  pose proof Korder_PreOrder M as H_PreOrder.
+  pose proof Korder_PreOrder as H_PreOrder.
   unfold iffp.
   rewrite sat_andp.
   split.
@@ -150,30 +150,28 @@ Proof.
     rewrite sat_emp in H2.
     assert (Korder u u) by reflexivity.
     specialize (H2 u H3).
-    unfold unit in H2.
     apply join_comm in H0.
+    rewrite unit_spec in H2.
     specialize (H2 _ _ H0).
     eapply sat_mono; eauto.
   + rewrite sat_impp; intros.
     rewrite sat_sepcon.
-    destruct (unit_exists M n) as [u [? ?]].
+    destruct (unit_exists n) as [u [? ?]].
     exists n, u.
     split; [| split]; auto.
     - apply join_comm; auto.
     - rewrite sat_emp; auto.
 Qed.
 
-Lemma sound_sepcon_elim {L: Language} {nL: NormalLanguage L} {pL: PropositionalLanguage L} {sL: SeparationLanguage L} {uSL: UnitarySeparationLanguage L} {SM: Semantics L} {pkS: PreKripkeSemantics L SM} {kiM: KripkeIntuitionisticModel L SM} {kiSM: KripkeIntuitionisticSemantics L SM} {dsSM: DownwardsSemantics L SM}:
+Lemma sound_sepcon_elim {L: Language} {nL: NormalLanguage L} {pL: PropositionalLanguage L} {SL: SeparationLanguage L} {MD: Model} {kMD: KripkeModel MD} (M: Kmodel) {kiM: KripkeIntuitionisticModel MD M} {SA: SeparationAlgebra MD M} {GC: GarbageCollectSeparationAlgebra MD M} {SM: Semantics L MD} {kiSM: KripkeIntuitionisticSemantics L MD M SM} {dsSM: DownwardsSemantics L MD M SM}:
   forall x y: expr,
-    forall M (join_as_Korder: forall M (m1 m2 m: Kworlds M), join m1 m2 m -> Korder m m1),
-      forall m, KRIPKE: M, m |= x * y --> x.
+    forall m, KRIPKE: M, m |= x * y --> x.
 Proof.
   intros.
-  pose proof Korder_PreOrder M as H_PreOrder.
+  pose proof Korder_PreOrder as H_PreOrder.
   rewrite sat_impp; intros.
   rewrite sat_sepcon in H0.
   destruct H0 as [m1 [m2 [? [? ?]]]].
-  apply join_as_Korder in H0.
+  apply join_has_order1 in H0.
   eapply sat_mono; eauto.
 Qed.
-  
