SeparationLogic/Sound_Upwards.v
@@ -5,6 +5,7 @@ Require Import Logic.MinimunLogic.MinimunLogic.
 Require Import Logic.PropositionalLogic.Syntax.
 Require Import Logic.SeparationLogic.Syntax.
 Require Import Logic.PropositionalLogic.KripkeSemantics.
+Require Import Logic.SeparationLogic.SeparationAlgebra.
 Require Import Logic.SeparationLogic.UpwardsSemantics.
 Require Import Logic.PropositionalLogic.IntuitionisticPropositionalLogic.
 Require Import Logic.SeparationLogic.SeparationLogic.
@@ -12,10 +13,11 @@ Require Import Logic.SeparationLogic.SeparationLogic.
 Local Open Scope logic_base.
 Local Open Scope PropositionalLogic.
 Local Open Scope SeparationLogic.
+Local Open Scope KripkeSemantics.
 
-Lemma sound_sepcon_comm {L: Language} {nL: NormalLanguage L} {pL: PropositionalLanguage L} {SL: SeparationLanguage L} {SM: Semantics L} {pkS: PreKripkeSemantics L SM} {kiM: KripkeIntuitionisticModel L SM} {kiSM: KripkeIntuitionisticSemantics L SM} {usSM: UpwardsSemantics L SM}:
+Lemma sound_sepcon_comm {L: Language} {nL: NormalLanguage L} {pL: PropositionalLanguage L} {SL: SeparationLanguage L} {MD: Model} {kMD: KripkeModel MD} (M: Kmodel) {kiM: KripkeIntuitionisticModel MD M} {SA: SeparationAlgebra MD M} {SM: Semantics L MD} {kiSM: KripkeIntuitionisticSemantics L MD M SM} {usSM: UpwardsSemantics L MD M SM}:
   forall x y: expr,
-    forall M m,
+    forall m,
       KRIPKE: M, m |= x * y --> y * x.
 Proof.
   intros.
@@ -27,13 +29,13 @@ Proof.
   apply join_comm; auto.
 Qed.
 
-Lemma sound_sepcon_assoc {L: Language} {nL: NormalLanguage L} {pL: PropositionalLanguage L} {sL: SeparationLanguage L} {SM: Semantics L} {pkS: PreKripkeSemantics L SM} {kiM: KripkeIntuitionisticModel L SM} {kiSM: KripkeIntuitionisticSemantics L SM} {usSM: UpwardsSemantics L SM}:
+Lemma sound_sepcon_assoc {L: Language} {nL: NormalLanguage L} {pL: PropositionalLanguage L} {SL: SeparationLanguage L} {MD: Model} {kMD: KripkeModel MD} (M: Kmodel) {kiM: KripkeIntuitionisticModel MD M} {SA: SeparationAlgebra MD M} {uSA: UpwardsClosedSeparationAlgebra MD M}{SM: Semantics L MD} {kiSM: KripkeIntuitionisticSemantics L MD M SM} {usSM: UpwardsSemantics L MD M SM}:
   forall x y z: expr,
-    forall M m,
+    forall m,
       KRIPKE: M, m |= x * (y * z) <--> (x * y) * z.
 Proof.
   intros.
-  pose proof Korder_PreOrder M as H_PreOrder.
+  pose proof Korder_PreOrder as H_PreOrder.
   unfold iffp.
   rewrite sat_andp.
   split; intros.
@@ -45,8 +47,8 @@ Proof.
     apply join_comm in H1.
     apply join_comm in H4.
     assert (Korder mx' mx') by reflexivity.
-    destruct (join_Korder M _ _ _ _ _ H1 H3 H7) as [n'' [? ?]].
-    destruct (join_assoc _ mz'' my'' mx' myz'' n'' H4 H8) as [mxy'' [? ?]].
+    destruct (join_Korder _ _ _ _ _ H1 H3 H7) as [n'' [? ?]].
+    destruct (join_assoc mz'' my'' mx' myz'' n'' H4 H8) as [mxy'' [? ?]].
     apply join_comm in H10.
     apply join_comm in H11.
     rewrite sat_sepcon.
@@ -63,8 +65,8 @@ Proof.
     rewrite sat_sepcon in H2.
     destruct H2 as [mxy'' [mx'' [my'' [? [? [? ?]]]]]].
     assert (Korder mz' mz') by reflexivity.
-    destruct (join_Korder M _ _ _ _ _ H1 H2 H7) as [n'' [? ?]].
-    destruct (join_assoc _ mx'' my'' mz' mxy'' n'' H4 H8) as [myz'' [? ?]].
+    destruct (join_Korder _ _ _ _ _ H1 H2 H7) as [n'' [? ?]].
+    destruct (join_assoc mx'' my'' mz' mxy'' n'' H4 H8) as [myz'' [? ?]].
     rewrite sat_sepcon.
     exists n'', mx'', myz''.
     split; [| split; [| split]]; auto.
@@ -75,13 +77,12 @@ Proof.
       reflexivity.
 Qed.
 
-Lemma sound_wand_sepcon_adjoint {L: Language} {nL: NormalLanguage L} {pL: PropositionalLanguage L} {sL: SeparationLanguage L} {SM: Semantics L} {pkS: PreKripkeSemantics L SM} {kiM: KripkeIntuitionisticModel L SM} {kiSM: KripkeIntuitionisticSemantics L SM} {usSM: UpwardsSemantics L SM}:
+Lemma sound_wand_sepcon_adjoint {L: Language} {nL: NormalLanguage L} {pL: PropositionalLanguage L} {SL: SeparationLanguage L} {MD: Model} {kMD: KripkeModel MD} (M: Kmodel) {kiM: KripkeIntuitionisticModel MD M} {SA: SeparationAlgebra MD M} {SM: Semantics L MD} {kiSM: KripkeIntuitionisticSemantics L MD M SM} {usSM: UpwardsSemantics L MD M SM}:
   forall x y z: expr,
-    forall M,
-     (forall m, KRIPKE: M, m |= x * y --> z) <-> (forall m, KRIPKE: M, m |= x --> (y -* z)).
+   (forall m, KRIPKE: M, m |= x * y --> z) <-> (forall m, KRIPKE: M, m |= x --> (y -* z)).
 Proof.
   intros.
-  pose proof Korder_PreOrder M as H_PreOrder.
+  pose proof Korder_PreOrder as H_PreOrder.
   split; intro.
   + assert (ASSU: forall m0 m1 m2 m, Korder m m0 -> join m1 m2 m0 -> KRIPKE: M, m1 |= x -> KRIPKE: M, m2 |= y -> KRIPKE: M, m |= z).
     Focus 1. {
@@ -115,15 +116,14 @@ Proof.
     eapply sat_mono; eauto.
 Qed.
 
-Lemma sound_sepcon_mono {L: Language} {nL: NormalLanguage L} {pL: PropositionalLanguage L} {sL: SeparationLanguage L} {SM: Semantics L} {pkS: PreKripkeSemantics L SM} {kiM: KripkeIntuitionisticModel L SM} {kiSM: KripkeIntuitionisticSemantics L SM} {usSM: UpwardsSemantics L SM}:
+Lemma sound_sepcon_mono {L: Language} {nL: NormalLanguage L} {pL: PropositionalLanguage L} {SL: SeparationLanguage L} {MD: Model} {kMD: KripkeModel MD} (M: Kmodel) {kiM: KripkeIntuitionisticModel MD M} {SA: SeparationAlgebra MD M} {SM: Semantics L MD} {kiSM: KripkeIntuitionisticSemantics L MD M SM} {usSM: UpwardsSemantics L MD M SM}:
   forall x1 x2 y1 y2: expr,
-    forall M,
-     (forall m, KRIPKE: M, m |= x1 --> x2) ->
-     (forall m, KRIPKE: M, m |= y1 --> y2) ->
-     (forall m, KRIPKE: M, m |= x1 * y1 --> x2 * y2).
+   (forall m, KRIPKE: M, m |= x1 --> x2) ->
+   (forall m, KRIPKE: M, m |= y1 --> y2) ->
+   (forall m, KRIPKE: M, m |= x1 * y1 --> x2 * y2).
 Proof.
   intros.
-  pose proof Korder_PreOrder M as H_PreOrder.
+  pose proof Korder_PreOrder as H_PreOrder.
   assert (ASSUx: forall m, KRIPKE: M, m |= x1 -> KRIPKE: M, m |= x2).
   Focus 1. {
     intros.
@@ -144,12 +144,12 @@ Proof.
   exists m0, m1, m2; auto.
 Qed.
 
-Lemma sound_sepcon_emp {L: Language} {nL: NormalLanguage L} {pL: PropositionalLanguage L} {sL: SeparationLanguage L} {uSL: UnitarySeparationLanguage L} {SM: Semantics L} {pkS: PreKripkeSemantics L SM} {kiM: KripkeIntuitionisticModel L SM} {kiSM: KripkeIntuitionisticSemantics L SM} {usSM: UpwardsSemantics L SM} {UusSM: UnitaryUpwardsSemantics L SM}:
+Lemma sound_sepcon_emp {L: Language} {nL: NormalLanguage L} {pL: PropositionalLanguage L} {SL: SeparationLanguage L} {uSL: UnitarySeparationLanguage L} {MD: Model} {kMD: KripkeModel MD} (M: Kmodel) {kiM: KripkeIntuitionisticModel MD M} {SA: SeparationAlgebra MD M} {USA: UnitarySeparationAlgebra MD M} {uSA: UpwardsClosedSeparationAlgebra MD M} {uUSA: UpwardsClosedUnitarySeparationAlgebra MD M} {SM: Semantics L MD} {kiSM: KripkeIntuitionisticSemantics L MD M SM} {usSM: UpwardsSemantics L MD M SM} {uUsSM: UnitaryUpwardsSemantics L MD M SM}:
   forall x: expr,
-    forall M m, KRIPKE: M, m |= x * emp <--> x.
+    forall m, KRIPKE: M, m |= x * emp <--> x.
 Proof.
   intros.
-  pose proof Korder_PreOrder M as H_PreOrder.
+  pose proof Korder_PreOrder as H_PreOrder.
   unfold iffp.
   rewrite sat_andp.
   split.
@@ -159,14 +159,16 @@ Proof.
     destruct H0 as [m'' [m' [u [? [? [? ?]]]]]].
     rewrite sat_emp in H2.
     destruct H2 as [u' [? ?]].
-    destruct (join_Korder M _ _ _ m' u' H0) as [m''' [? ?]]; [reflexivity | auto |].
-    apply join_comm in H4; apply H3 in H4.
+    destruct (join_Korder _ _ _ m' u' H0) as [m''' [? ?]]; [reflexivity | auto |].
+    apply join_comm in H4.
+    rewrite unit_spec in H3.
+    apply H3 in H4.
     subst m'''.
     eapply sat_mono; eauto.
     eapply sat_mono; eauto.
   + rewrite sat_impp; intros.
     rewrite sat_sepcon.
-    destruct (unit_exists M n) as [u [? ?]].
+    destruct (unit_exists n) as [u [? ?]].
     exists n, n, u.
     split; [| split; [| split]]; auto.
     - reflexivity.
@@ -176,18 +178,16 @@ Proof.
       reflexivity.
 Qed.
 
-Lemma sound_sepcon_elim {L: Language} {nL: NormalLanguage L} {pL: PropositionalLanguage L} {sL: SeparationLanguage L} {uSL: UnitarySeparationLanguage L} {SM: Semantics L} {pkS: PreKripkeSemantics L SM} {kiM: KripkeIntuitionisticModel L SM} {kiSM: KripkeIntuitionisticSemantics L SM} {usSM: UpwardsSemantics L SM}:
+Lemma sound_sepcon_elim {L: Language} {nL: NormalLanguage L} {pL: PropositionalLanguage L} {SL: SeparationLanguage L} {MD: Model} {kMD: KripkeModel MD} (M: Kmodel) {kiM: KripkeIntuitionisticModel MD M} {SA: SeparationAlgebra MD M} {GC: GarbageCollectSeparationAlgebra MD M} {SM: Semantics L MD} {kiSM: KripkeIntuitionisticSemantics L MD M SM} {usSM: UpwardsSemantics L MD M SM}:
   forall x y: expr,
-    forall M (join_as_Korder: forall M (m1 m2 m: Kworlds M), join m1 m2 m -> Korder m m1),
-      forall m, KRIPKE: M, m |= x * y --> x.
+    forall m, KRIPKE: M, m |= x * y --> x.
 Proof.
   intros.
-  pose proof Korder_PreOrder M as H_PreOrder.
+  pose proof Korder_PreOrder as H_PreOrder.
   rewrite sat_impp; intros.
   rewrite sat_sepcon in H0.
   destruct H0 as [m0 [m1 [m2 [? [? [? ?]]]]]].
-  apply join_as_Korder in H1.
+  apply join_has_order1 in H1.
   eapply sat_mono; eauto.
   eapply sat_mono; eauto.
 Qed.
-  
