SeparationLogic/Upwards2Downwards.v
@@ -5,6 +5,7 @@ Require Import Logic.MinimunLogic.MinimunLogic.
 Require Import Logic.PropositionalLogic.Syntax.
 Require Import Logic.SeparationLogic.Syntax.
 Require Import Logic.PropositionalLogic.KripkeSemantics.
+Require Import Logic.SeparationLogic.SeparationAlgebra.
 Require Import Logic.SeparationLogic.UpwardsSemantics.
 Require Import Logic.SeparationLogic.DownwardsSemantics.
 
@@ -12,28 +13,35 @@ Local Open Scope logic_base.
 Local Open Scope PropositionalLogic.
 Local Open Scope SeparationLogic.
 
-Definition u2d_sSM {L: Language} {nL: NormalLanguage L} {pL: PropositionalLanguage L} {SL: SeparationLanguage L} {SM: Semantics L} {pkSM: PreKripkeSemantics L SM} {kiM: KripkeIntuitionisticModel L SM} {kiSM: KripkeIntuitionisticSemantics L SM} (usSM: UpwardsSemantics L SM): DownwardsSemantics L SM.
-  refine (Build_DownwardsSemantics _ _ _ _ _ _ _ _ (fun M (m1 m2 m: Kworlds M) => exists n, Korder m n /\ UpwardsSemantics.join m1 m2 n) _ _ _ _ _).
-  + (* join_comm *)
-    intros.
+Section Upwards2Downwards.
+
+Context {MD: Model} {kMD: KripkeModel MD} {kiMD: KripkeIntuitionisticModel MD} {SA: SeparationAlgebra MD}.
+
+Definition u2d_SA: SeparationAlgebra MD.
+  apply (Build_SeparationAlgebra _ _ (fun M (m1 m2 m: Kworlds M) => exists n, Korder m n /\ join m1 m2 n)).
+  + intros.
     destruct H as [n [? ?]].
     exists n.
     split; auto.
-    apply UpwardsSemantics.join_comm; auto.
-  + (* join_assoc *)
-    intros.
+    apply join_comm; auto.
+  + intros.
     pose proof Korder_PreOrder M as H_PreOrder.
     rename mx into mx', my into my', mz into mz'.
     destruct H as [mxy' [? ?]].
     destruct H0 as [mxyz' [? ?]].
-    destruct (UpwardsSemantics.join_Korder M _ _ _ _ mz' H2 H) as [mxyz'' [? ?]]; [reflexivity |].
-    destruct (UpwardsSemantics.join_assoc M _ _ _ _ _ H1 H3) as [myz' [? ?]].
+    destruct (join_Korder _ _ _ _ mz' H2 H) as [mxyz'' [? ?]]; [reflexivity |].
+    destruct (join_assoc _ _ _ _ _ H1 H3) as [myz' [? ?]].
     exists myz'.
     split.
     - exists myz'; split; auto.
       reflexivity.
     - exists mxyz''; split; auto.
       etransitivity; eauto.
+
+Context {L: Language} {nL: NormalLanguage L} {pL: PropositionalLanguage L} {SL: SeparationLanguage L}  {SM: Semantics L MD} {kiSM: KripkeIntuitionisticSemantics L MD SM} {dsSM: DownwardsSemantics L MD SM}.
+
+Definition u2d_sSM {L: Language} {nL: NormalLanguage L} {pL: PropositionalLanguage L} {SL: SeparationLanguage L} {SM: Semantics L} {pkSM: PreKripkeSemantics L SM} {kiM: KripkeIntuitionisticModel L SM} {kiSM: KripkeIntuitionisticSemantics L SM} (usSM: UpwardsSemantics L SM): DownwardsSemantics L SM.
+  refine (Build_DownwardsSemantics _ _ _ _ _ _ _ _ (fun M (m1 m2 m: Kworlds M) => exists n, Korder m n /\ UpwardsSemantics.join m1 m2 n) _ _ _ _ _).
   + (* join_Korder *)
     intros.
     pose proof Korder_PreOrder M as H_PreOrder.
